@prefix desm: <http://desmsolutions.org/ns/> .
@prefix dct: <http://purl.org/dc/terms/> .
@prefix owl: <http://www.w3.org/2002/07/owl#> .
@prefix rdf: <http://www.w3.org/1999/02/22-rdf-syntax-ns#> .
@prefix rdfs: <http://www.w3.org/2000/01/rdf-schema#> .
@prefix sdo: <http://schema.org/> .
@prefix skos: <http://www.w3.org/2004/02/skos/core#> .
@prefix xml: <http://www.w3.org/XML/1998/namespace> .
@prefix xsd: <http://www.w3.org/2001/XMLSchema#> .


desm:AbstractClassMapping a rdfs:Class ;
    rdfs:label "Abstract Class Mapping"@en ;
    rdfs:comment "Resource describing mappings by one or more Data Standards Organizations (DSOs) to a single abstract class."@en ;
    rdfs:isDefinedBy desm:
    .
desm:MappingConfiguration a rdfs:Class ;
    rdfs:label "Mapping Configuration Set"@en ;
    rdfs:comment "Resource identifying the form and aggregation of one or more mappings of one or more Abstract Class created by one or more Data Standards Organizations (DSOs)."@en ;
    rdfs:isDefinedBy desm:
    .
desm:Agent a rdfs:Class ;
    rdfs:label "Agent"@en ;
    rdfs:comment "Personnel engaged in the process of crosswalking terms"@en ;
    rdfs:isDefinedBy desm:
    .
rdfs:Class a rdfs:Class ;
    rdfs:label "Class"@en ;
    rdfs:comment "Type or class of resource to which properties are related."@en ;
    skos:scopeNote "Related to, but not the same as rdfs:Class."@en ;
    rdfs:isDefinedBy rdfs:
    .
skos:Concept a rdfs:Class ;
    rdfs:label "Concept"@en ;
    rdfs:comment "An idea or notion; a unit of thought."@en ;
    rdfs:isDefinedBy skos:
    .
skos:ConceptScheme a rdfs:Class ;
    rdfs:label "Concept Scheme"@en ;
    rdfs:comment "A set of concepts, optionally including statements about semantic relationships between those concepts."@en ;
    skos:scopeNote "A concept scheme may be defined to include concepts from different sources."@en ;
    rdfs:isDefinedBy skos:
    .
desm:DSO a rdfs:Class ;
    rdfs:label "Data Standards Organization"@en ;
    rdfs:comment "Organization or person responsible for creating or making available a de facto or de jure data standard being crosswalked in a project."@en ;
    rdfs:isDefinedBy desm:
    .
rdf:Property a rdfs:Class ;
    rdfs:label "Property"@en ;
    rdfs:comment "Property in a cross walk crosswalked to a propery in the spine."@en ;
    skos:scopeNote "Crosswalks map a properties from the DSOs' schemas to properties in the synthetic spine."@en ;
    rdfs:isDefinedBy rdf:
    .
desm:Schema a rdfs:Class ;
    rdfs:label "Schema"@en ;
    rdfs:comment "Resource describing controlled concepts or enumerations."@en ;
    rdfs:isDefinedBy desm:
    .
desm:administrator a rdf:Property ;
    rdfs:label "Administrator"@en ;
    rdfs:comment "Agent with administrative duties."@en ;
    rdfs:domain desm:DSO ;
    rdfs:range desm:Agent;
    rdfs:isDefinedBy desm:
    .
desm:asbtractClassModeled a rdf:Property ;
    rdfs:label "Abstract Class Modeled"@en ;
    rdfs:comment "Instance of the abstract class used by a term mapping."@en ;
    skos:scopeNote "References a specific abstract class instance in the SKOS concept scheme for abstract classes identified in the configuration profile being used."@en ;
    rdfs:domain desm:AbstractClassMapping;
    rdfs:range skos:Concept;
    rdfs:isDefinedBy desm:
    .
desm:asbtractClassType a rdf:Property ;
    rdfs:label "Abstract Class Type Scheme"@en ;
    rdfs:comment "The abstract class concept scheme used in a mapping project"@en ;
    rdfs:domain desm:AbstractClassSet;
    rdfs:range skos:COnceptScheme;
    rdfs:isDefinedBy desm:
    .
skos:broader a rdf:Property ;
    rdfs:label "Has Broader"@en ;
    rdfs:comment "Broader concepts are typically rendered as parents in a concept hierarchy (tree)."@en ;
    rdfs:domain skos:Concept ;
    rdfs:range skos:Concept ;
    rdfs:isDefinedBy skos:
    .
dct:created a rdf:Property ;
    rdfs:label "Date Created"@en ;
    rdfs:comment "Date of creation of the resource."@en ;
    rdfs:domain desm:AbstractClassMapping, desm:AbstractClassSet;
    rdfs:range xsd:date;
    rdfs:isDefinedBy dct:
    .
dct:creator a rdf:Property ;
    rdfs:label "Creator"@en ;
    rdfs:comment "An entity responsible for making the resource."@en ;
    skos:scopeNote ""@en ;
    rdfs:domain desm:Schema ;
    rdfs:range desm:Agent ;
    rdfs:isDefinedBy dct:
    .
sdo:email a rdf:Property ;
    rdfs:label "email"@en ;
    rdfs:comment "Email address."@en ;
    rdfs:domain desm:Agent ;
    rdfs:range xsd:string ;
    rdfs:isDefinedBy sdo:
    .
desm:githubHandle a rdf:Property ;
    rdfs:label "GitHub handle"@en ;
    rdfs:comment "GitHub username."@en ;
    rdfs:domain desm:Agent;
    rdfs:range xsd:string ;
    rdfs:isDefinedBy desm:
    .
desm:hasDSO a rdf:Property ;
    rdfs:label "Has DSO"@en ;
    rdfs:comment "DSO participating in one or more asbtract class mappings in this project."@en ;
    rdfs:domain desm:MappingCOnfiguration;
    rdfs:range desm:DSO ;
    rdfs:isDefinedBy desm:
    .
dct:hasPart a rdf:Property ;
    rdfs:label "Has Part"@en ;
    rdfs:comment "Related resource that is included either physically or logically in the described resource."@en ;
    rdfs:domain desm:AbstractClassSet ,
        desm:AbstractCLassMapping ;
    rdfs:range desm:AbstractClassMapping ,
        desm:TermMapping ;
    rdfs:isDefinedBy dct:
    .
desm:hasProperty a rdf:Property ;
    rdfs:label "Has Property"@en ;
    rdfs:comment "Property of a particular schema."@en ;
    rdfs:domain desm:Schema ;
    rdfs:range rdf:Property;
    rdfs:isDefinedBy desm:
    .
desm:hasSchema a rdf:Property ;
    rdfs:label "Has Schema"@en ;
    rdfs:comment "Schema in which this property is defined."@en ;
    rdfs:domain rdf:Property ;
    rdfs:range desm:Schema ;
    rdfs:isDefinedBy desm:
    .
desm:hasScheme a rdf:Property ;
    rdfs:label "Has Scheme"@en ;
    rdfs:comment "Concept Scheme that belongs to this Data Standards Organization."@en ;
    rdfs:domain desm:DSO ;
    rdfs:range skos:ConceptScheme ;
    rdfs:isDefinedBy desm:
    .
desm:hasTermMapping a rdf:Property ;
    rdfs:label "Has Term Mapping"@en ;
    rdfs:comment "Relates a property to a term mapping in which it is included."@en ;
    rdfs:domain rdf:Property ;
    rdfs:range desm:TermMapping ;
    rdfs:isDefinedBy desm:
    .
skos:hasTopConcept a rdf:Property ;
    rdfs:label "hasTopCOncept"@en ;
    rdfs:comment "Relates, by convention, a concept scheme to a concept which is topmost in the broader\/narrower concept hierarchies for that scheme, providing an entry point to these hierarchies."@en ;
    rdfs:domain skos:ConceptScheme ;
    rdfs:range skos:Concept ;
    rdfs:isDefinedBy skos:
    .
desm:inSchema a rdf:Property ;
    rdfs:label "In Schema"@en ;
    rdfs:comment "Relates a property to a scheme in which it is included."@en ;
    rdfs:domain rdf:Property ;
    rdfs:range desm:Schema ;
    rdfs:isDefinedBy desm:
    .
skos:inScheme a rdf:Property ;
    rdfs:label "In Scheme"@en ;
    rdfs:comment "Relates a resource (for example a concept) to a concept scheme in which it is included."@en ;
    rdfs:domain skos:Concept ;
    rdfs:range skos:ConceptScheme ;
    rdfs:isDefinedBy skos:
    .
dct:isPartOf a rdf:Property ;
    rdfs:label "Is Part Of"@en ;
    rdfs:comment "A related resource in which the described resource is physically or logically included."@en ;
    rdfs:domain desm:TermMapping ,
        desm:AbstractClassMapping ;
    rdfs:range  desm:AbstractMapping ,
        desm:AbstractClassSet ;
    rdfs:isDefinedBy dct:
    .
desm:issue a rdf:Property ;
    rdfs:label "Issue"@en ;
    rdfs:comment "Recording of an issue with mapping a property to another property."@en ;
    rdfs:domain desm:TermMapping ;
    rdfs:range rdf:langString ;
    rdfs:isDefinedBy desm:
    .
rdfs:label a rdf:Property ;
    rdfs:label "Human-readable version of the name of a resource."@en ;
    rdfs:domain rdf:Property ,
        rdfs:Class ;
    rdfs:range rdf:langString ;
    rdfs:isDefinedBy rdfs:
    .
desm:mappedTerm a rdf:Property ;
    rdfs:label "Mapped Term"@en ;
    rdfs:comment "Property being mapped to a spine property."@en ;
    rdfs:domain desm:TermMapping ;
    rdfs:range rdf:Property ;
    rdfs:isDefinedBy desm:
    .
desm:mapper a rdf:Property ;
    rdfs:label "Mapper"@en ;
    rdfs:comment "An agent adminitering or performing a mapping or crosswalk."@en ;
    rdfs:domain desm:DSO ;
    rdfs:range desm:Agent ;
    rdfs:isDefinedBy desm:
    .
desm:mappingPredicate a rdf:Property ;
    rdfs:label "Mapping Predicate"@en ;
    rdfs:comment "Concept identifying the relationship between two properties being mapped."@en ;
    rdfs:domain desm:TermMapping ;
    rdfs:range skos:Concept ;
    rdfs:isDefinedBy desm:
    .
desm:mappingPredicateType a rdf:Property ;
    rdfs:label "Mapping Predicate Type"@en ;
    rdfs:comment "Concept scheme defining mapping predicate types."@en ;
    rdfs:domain desm:AbstractCLassSet ;
    rdfs:range skos:ConceptScheme ;
    rdfs:isDefinedBy desm:
    .
sdo:name a rdf:Property ;
    rdfs:label "Name"@en ;
    rdfs:comment "The name of the item."@en ;
    rdfs:domain desm:Agent ;
    rdfs:range rdf:langString ;
    rdfs:isDefinedBy sdo:
    .
skos:narrower a rdf:Property ;
    rdfs:label "Narrower"@en ;
    rdfs:comment "Narrower concepts are typically rendered as children in a concept hierarchy (tree)."@en ;
    rdfs:domain skos:Concept ;
    rdfs:range skos:Concept ;
    rdfs:isDefinedBy skos:
    .
desm:range a rdf:Property ;
    rdfs:label "Range"@en ;
    rdfs:comment "Property to used to state that the values of a property are instances of one or more classes."@en ;
    rdfs:domain rdf:Property;
    rdfs:range skos:Concept ,
        desm:Class ;
    rdfs:isDefinedBy desm:
    .
desm:relatedSchema a rdf:Property ;
    rdfs:label "Related Schema"@en ;
    rdfs:comment "Schema to which a concept scheme provides property values."@en ;
    rdfs:domain skos:ConceptSCheme ;
    rdfs:range desm:Schema ;
    rdfs:isDefinedBy desm:
    .
desm:role a rdf:Property ;
    rdfs:label "Role"@en ;
    rdfs:comment "Functon or job of an agent."@en ;
    rdfs:domain desm:Agent ;
    rdfs:range rdf:langString ;
    rdfs:isDefinedBy desm:
    .
desm:sourcePath a rdf:Property ;
    rdfs:label "Source Path"@en ;
    rdfs:comment "Property or class path in a schema."@en ;
    rdfs:domain rdf:Property ;
    rdfs:range xsd:string ;
    rdfs:isDefinedBy desm:
    .
desm:spineTerm a rdf:Property ;
    rdfs:label "Spine Term"@en ;
    rdfs:comment "Property of the synthetic spine generated during the mapping process."@en ;
    rdfs:domain desm:TermMapping ;
    rdfs:range rdf:Property ;
    rdfs:isDefinedBy desm:
    .