@prefix dcterms: <http://purl.org/dc/terms/> .
@prefix desm: <https://desmsolutions.org/ns/> .
@prefix skos: <http://www.w3.org/2004/02/skos/core#> .
@prefix xsd: <http://www.w3.org/2001/XMLSchema#> .

<http://desmsolutions.org/concepts/identical> a skos:Concept ;
    skos:inScheme <http://desmsolutions.org/concepts/desmMappingPredicates> ;
    skos:prefLabel "Identical"@en-us ;
	skos:definition "The definition is identical in wording and intent."@en-US ;
    desm:weight 5 .

<http://desmsolutions.org/concepts/reworded> a skos:Concept ;
    skos:inScheme <http://desmsolutions.org/concepts/desmMappingPredicates> ;
    skos:prefLabel "Reworded"@en-us ;
	skos:definition "The definition is identical in intent but reworded; the properties are equivalent."@en-US ;
    desm:weight 5 .

<http://desmsolutions.org/concepts/similar> a skos:Concept ;
    skos:inScheme <http://desmsolutions.org/concepts/desmMappingPredicates> ;
    skos:prefLabel "Similar"@en-us ;
	skos:definition "The definition is similar in intent, but with significant wording differences."@en-US ;
    desm:weight 4 .

<http://desmsolutions.org/concepts/transformed> a skos:Concept ;
    skos:inScheme <http://desmsolutions.org/concepts/desmMappingPredicates> ;
    skos:prefLabel "Transformed"@en-us ;
	skos:definition "A simple data transform will yield a value for the spine term; for example, concatenating values from several properties being mapped. Describe the transform in a comment on the alignment."@en-US ;
    desm:weight 4 .

<http://desmsolutions.org/concepts/aggregated> a skos:Concept ;
    skos:inScheme <http://desmsolutions.org/concepts/desmMappingPredicates> ;
    skos:prefLabel "aggregated"@en-us ;
	skos:definition "The term in the spine aggregates terms from the mapped schema."@en-US ;
    desm:weight 3 .

<http://desmsolutions.org/concepts/disaggregated> a skos:Concept ;
    skos:inScheme <http://desmsolutions.org/concepts/desmMappingPredicates> ;
    skos:prefLabel "aggregated"@en-us ;
	skos:definition "The term in the spine disaggregates terms from the mapped schema."@en-US ;
    desm:weight 3 .

<http://desmsolutions.org/concepts/concept> a skos:Concept ;
    skos:inScheme <http://desmsolutions.org/concepts/desmMappingPredicates> ;
    skos:prefLabel "Concept"@en-us ;
	skos:definition "The definition is related only at a conceptual level, no simple transformation can render the data from one to the other."@en-US ;
    desm:weight 2 .

<http://desmsolutions.org/concepts/noMatch> a skos:Concept ;
    skos:inScheme <http://desmsolutions.org/concepts/desmMappingPredicates> ;
    skos:prefLabel "No Match"@en-us ;
	skos:definition "There is no match for the spine term in the schema being mapped."@en-US ;
    desm:weight 0 .

<http://desmsolutions.org/concepts/notApplicable> a skos:Concept ;
    skos:inScheme <http://desmsolutions.org/concepts/desmMappingPredicates> ;
    skos:prefLabel "Not Applicable"@en-us ;
	skos:definition "For some reason this term is not relevant to the mapping."@en-US ;
    desm:weight 0 .

<http://desmsolutions.org/concepts/Issue> a skos:Concept ;
    skos:inScheme <http://desmsolutions.org/concepts/desmMappingPredicates> ;
    skos:prefLabel "Issue"@en-us ;
	skos:definition "We have a problem."@en-US ;
    desm:weight 0 .

<http://desmsolutions.org/concepts/desmMappingPredicates> a skos:ConceptScheme ;
    dcterms:created "2022-10-31"^^xsd:date ;
    dcterms:creator <http://people.pjjk.net/phil> ;
    dcterms:description "This concept scheme identifies the mapping predicates used by the DESM Pilot Project."@en-us ;
    dcterms:title "DESM Pilot Project Mapping Predicates"@en-us ;
    skos:hasTopConcept
        <http://desmsolutions.org/concepts/concept> ,
        <http://desmsolutions.org/concepts/reworded> ,
        <http://desmsolutions.org/concepts/identical> ,
        <http://desmsolutions.org/concepts/similar> ,
        <http://desmsolutions.org/concepts/notApplicable> ,
        <http://desmsolutions.org/concepts/aggregated> ,
        <http://desmsolutions.org/concepts/noMatch> ,
        <http://desmsolutions.org/concepts/issue> ,
        <http://desmsolutions.org/concepts/disaggregated>,
        <http://desmsolutions.org/concepts/transformed>
.
