@prefix dcterms: <http://purl.org/dc/terms/> .
@prefix skos: <http://www.w3.org/2004/02/skos/core#> .
@prefix xsd: <http://www.w3.org/2001/XMLSchema#> .
@prefix mcac: <https://raw.githubusercontent.com/CredentialEngine/desm/main/concepts/pilotMappingPredicates.ttl#> .

mcac:Assertion a skos:Concept ;
    skos:inScheme mcac: ;
    skos:definition "Main object of a verifiable credential that asserts statements about the issuing of the credential to an individual."@en ;
    skos:prefLabel "Assertion"@en .

mcac:MicrocredentialClaimed a skos:Concept ;
    skos:inScheme mcac: ;
    skos:definition "Definition or specification of the micro-credential that can be issued to an agent."@en ;
    skos:prefLabel "Micro-credential claimed"@en .

mcac:Issuer a skos:Concept ;
    skos:inScheme mcac: ;
    skos:definition "Agent (typically an Organization or Person) agent that makes the assertion about the subject."@en ;
    skos:prefLabel "Issuer"@en .

mcac:OwnerOfferer a skos:Concept ;
    skos:inScheme mcac: ;
    skos:definition "Agent (typically an Organization or Person) that owns the rights to, or offers the microcredential claimed."@en ;
    skos:prefLabel "Owner/Offerer"@en .

<http://desm.org/concepts/mappingClasses> a skos:ConceptScheme ;
    dcterms:created "2022-10-31"^^xsd:date ;
    dcterms:creator <https://people.pjjk.net/phil> ;
    dcterms:description "This concept scheme identifies the abstract mapping classes used by the DESM pilot project."@en-us ;
    dcterms:title "DESM Pilot Project Abstract Mapping Classes"@en-us ;
    skos:hasTopConcept mcac:Assertion , 
        mcac:MicrocredentialClaimed , 
        mcac:Issuer ,
        mcac:OwnerOfferer .