{
  "@context": {
    "id": "@id",
    "type": "@type",
    "dct": "http://purl.org/dc/terms/",
    "desm": "https://github.com/t3-innovation-network/desm/tree/main/schemas/desmSchema/",
    "rdf": "http://www.w3.org/1999/02/22-rdf-syntax-ns#",
    "rdfs": "http://www.w3.org/2000/01/rdf-schema#",
    "skos": "http://www.w3.org/2004/02/skos/core#",
    "sdo": "sdo:",
    "xsd": "http://www.w3.org/2001/XMLSchema#" ,
    "AbstractClassMapping": {"@id": "desm:AbstractClassMapping"} ,
    "AbstractClassSet": {"@id": "desm:AbstractClassSet"} ,
    "Agent": {"@id": "desm:Agent"} ,
    "Class": {"@id": "rdfs:Class"} ,
    "Concept": {"@id": "skos:Concept"} ,
    "ConceptScheme": {"@id": "skos:ConceptScheme"} ,
    "DSO": {"@id": "desm:DSO"} ,
    "Schema": {"@id": "desm:Schema"} ,
    "Property": {"@id": "rdf:Property"} ,
    "abstractClassModeled": {"@id": "desm:abstractClassModeled", "@type": "@id"} ,
    "abstractClassType": {"@id": "desm:abstractClassType", "@type": "@id"} ,
    "administrator": {"@id": "desm:administrator", "@type": "@id"} ,
    "broader": {"@id": "skos:broader", "@type": "@id"} ,
    "created": {"@id": "dct:created", "@type": "xsd:date"} ,
    "creator": {"@id": "dct:creator", "@type": "@id"} ,
    "description": {"@id": "dct:description", "@container": "@language"} ,
    "email": {"@id": "sdo:email", "@type": "xsd:string"} ,
    "githubHandle": {"@id": "desm:githubHandle", "@type": "xsd:string"} ,
    "hasDSO": {"@id": "desm:hasDSO", "@type": "@id"} , 
    "hasPart": {"@id": "dct:hasPart", "@type": "@id"} ,
    "hasProperty": {"@id": "desm:hasProperty", "@type": "@id"} ,
    "hasSchema": {"@id": "desm:hasSchema", "@type": "@id"} ,
    "hasScheme": {"@id": "desm:hasScheme", "@type": "@id"} ,
    "hasTermMapping": {"@id": "desm:hasTermMapping", "@type": "@id"} ,   
    "hasTopConcept": {"@id": "skos:hasTopConcept", "@type": "@id"} ,
    "inSchema": {"@id": "desm:inSchema", "@type": "@id"} ,
    "inScheme": {"@id": "skos:inScheme", "@type": "@id"} ,
    "isPartOf": {"@id": "dct:isPartOf", "@type": "@id"} ,
    "issue": {"@id": "desm:issue", "@container": "@language"} ,
    "label": {"@id": "rdfs:label", "@container": "@language"} ,
    "mappedTerm": {"@id": "desm:mappedTerm", "@type": "@id"} ,
    "mapper": {"@id": "desm:mapper", "@type": "@id"} ,
    "mappingPredicate": {"@id": "desm:mappingPredicate", "@type": "@id"} ,
    "name": {"@id": "sdo:name", "@container": "@language"} ,
    "narrower": {"@id": "skos:narrower", "@type": "@id"} ,
    "prefLabel": {"@id": "skos:prefLabel", "@container": "@language"} ,
    "range": {"@id": "desm:range", "@type": "@id"} ,
    "relatedSchema": {"@id": "desm:relatedSchema", "@type": "@id"} ,
    "role": {"@id": "desm:role", "@type": "@id"} ,
    "sourcePath": {"@id": "desm:sourcePath", "@type": "xsd:string"} ,
    "spineTerm": {"@id": "desm:spineTerm", "@type": "xsd:string"} ,
    "title": {"@id": "dcterms:title", "@container": "@language"}
  },
  
  "@graph": 
    [
        {
            "@id": "desm:AbstractClassMapping",
            "@type": "rdfs:Class",
            "rdfs:label": {"en": "Abstract Class Mapping"}, 
            "rdfs:comment": {"en": "Resource describing mappings by one or more Data Standards Organizations (DSOs) to a single abstract class."},
            "rdfs:isDefinedBy": "desm:"
        },
        {
            "@id": "desm:Agent",
            "@type": "rdfs:Class",
            "rdfs:label": {"en": "Agent"},
            "rdfs:comment": {"en": "Personnel engaged in the process of crosswalking terms"},
            "rdfs:isDefinedBy": "desm:"
        },
        {
            "@id": "rdfs:Class",
            "@type": "rdfs:Class",
            "rdfs:label": {"en": "Class"},
            "rdfs:comment": {"en": "Type or class of resource to which properties are related."},
            "skos:scopeNote": {"en": "Related to, but not the same as rdfs:Class."},
            "rdfs:isDefinedBy": "rdfs:"
        },
        {
            "@id": "skos:Concept",
            "@type": "rdfs:Class",
            "rdfs:label": {"en": "Concept"},
            "skos:comment": {"en": "An idea or notion; a unit of thought."},
            "rdfs:isDefinedBy": "skos:"
        },
        {
            "@id": "skos:ConceptScheme",
            "@type": "rdfs:Class",
            "rdfs:label": {"en": "Concept Scheme"},
            "rdfs:comment": {"en": "A set of concepts, optionally including statements about semantic relationships between those concepts."},
            "skos:scopeNote": {"en": "A concept scheme may be defined to include concepts from different sources."}, 
            "rdfs:isDefinedBy": "skos:"
        },
        {
            "@id": "desm:DSO",
            "@type": "rdfs:Class",
            "rdfs:label": {"en": "Data Standards Organization"},
            "rdfs:comment": {"en": "Organization or person responsible for creating or making available a de facto or de jure data standard being crosswalked in a project."},
            "rdfs:isDefinedBy": "desm:"
        },
        {
            "@id": "desm:MappingConfiguration",
            "@type": "rdfs:Class",
            "rdfs:label": {"en": "Mapping Configuration"},
            "rdfs:comment": {"en": "Resource identifying the form and aggregation of one or more mappings of one or more Abstract Class created by one or more Data Standards Organizations (DSOs)."},
            "rdfs:isDefinedBy": "desm:"
        },
        {
            "@id": "rdf:Property",
            "@type": "rdfs:Class",
            "rdfs:label": {"en": "Property"},
            "rdfs:comment": {"en": "Property in a cross walk crosswalked to a propery in the spine."},
            "skos:scopeNote": {"en": "Crosswalks map a properties from the DSOs' schemas to properties in the synthetic spine."},
            "rdfs:isDefinedBy": "rdf:"
        },
        {
            "@id": "desm:Schema",
            "@type": "rdfs:Class",
            "rdfs:label": {"en": "Resource describing controlled concepts or enumerations."},
            "rdfs:isDefinedBy": "desm:"
        },
                {
            "@id": "desm:administrator",
            "@type": "rdf:Property",
            "rdfs:label": {"en": "Administrator"},
            "rdfs:comment": {"en": "Agent with administrative duties."},
            "rdfs:domain": "desm:DSO",
            "rdfs:range": "desm:Agent",
            "rdfs:isDefinedBy": "desm:"
        },
        {
            "@id": "desm:asbtractClassModeled",
            "@type": "rdf:Property",
            "rdfs:label": {"en": "Abstract Class Modeled"},
            "rdfs:comment": {"en": "Instance of the abstract class used by a term mapping."},
            "skos:scopeNote": {"en": "References a specific abstract class instance in the SKOS concept scheme for abstract classes identified in the configuration profile being used."},
            "rdfs:domain": "desm:AbstractClassMapping",
            "rdfs:range": "skos:Concept",
            "rdfs:isDefinedBy": "desm:"
        },
        {
            "@id": "desm:asbtractClassType",
            "@type": "rdf:Property",
            "rdfs:label": {"en": "Abstract Class Type Scheme"},
            "rdfs:comment": {"en": "The abstract class concept scheme used in a mapping project"},
            "rdfs:domain": "desm:AbstractClassSet",
            "rdfs:range": "skos:COnceptScheme",
            "rdfs:isDefinedBy": "desm:"
        },
        {
            "@id": "skos:broader",
            "@type": "rdf:Property",
            "rdfs:label": {"en": "Has Broader"},
            "rdfs:comment": {"en": "Broader concepts are typically rendered as parents in a concept hierarchy (tree)."},
            "rdfs:domain": "skos:Concept",
            "rdfs:range": "skos:Concept",
            "rdfs:isDefinedBy": "skos:"
        },
        {
            "@id": "dct:created",
            "@type": "rdf:Property",
            "rdfs:label": {"en": "Date Created"},
            "rdfs:comment": {"en": "Date of creation of the resource."},
            "rdfs:domain": [
                "desm:AbstractClassMapping",
                "desm:AbstractClassSet"
            ],
            "rdfs:range": "xsd:date",
            "rdfs:isDefinedBy": "dct:"
        },
        {
            "@id": "dct:creator",
            "@type": "rdf:Property",
            "rdfs:label": {"en": "Creator"},
            "rdfs:comment": {"en": "An entity responsible for making the resource."},
            "rdfs:domain": "desm:Schema",
            "rdfs:range": "desm:Agent",
            "rdfs:isDefinedBy": "dct:"
        },
        {
            "@id": "sdo:email",
            "@type": "rdf:Property",
            "rdfs:label": {"en": "email"},
            "rdfs:comment": {"en": "Email address."},
            "rdfs:domain": "desm:Agent",
            "rdfs:range": "xsd:string",
            "rdfs:isDefinedBy": "sdo:"
        },
        {
            "@id": "desm:githubHandle",
            "@type": "rdf:Property",
            "rdfs:label": {"en": "GitHub handle"},
            "rdfs:comment": {"en": "GitHub username."},
            "rdfs:domain": "desm:Agent",
            "rdfs:range": "xsd:string",
            "rdfs:isDefinedBy": "desm:"
        },
        {
            "@id": "desm:hasDSO",
            "@type": "rdf:Property",
            "rdfs:label": {"en": "Has DSO"},
            "rdfs:comment": {"en": "DSO participating in one or more asbtract class mappings in this project."},
            "rdfs:domain": "desm:MappingConfiguration",
            "rdfs:range": "desm:DSO",
            "rdfs:isDefinedBy": "desm:"
        },
        {
            "@id": "dct:hasPart",
            "@type": "rdf:Property",
            "rdfs:label": {"en": "Has Part"},
            "rdfs:comment": {"en": "Related resource that is included either physically or logically in the described resource."},
            "rdfs:domain": [
                "desm:AbstractClassSet",
                "desm:AbstractCLassMapping"
            ],
            "rdfs:range": [
                "desm:AbstractClassMapping",
                "desm:TermMapping"
            ],
            "rdfs:isDefinedBy": "dct:"
        },        
        {
            "@id": "desm:hasProperty",
            "@type": "rdf:Property",
            "rdfs:label": {"en": "Has Property"},
            "rdfs:comment": {"en": "Property of a particular schema."},
            "rdfs:domain": "desm:Schema",
            "rdfs:range": "rdf:Property",
            "rdfs:isDefinedBy": "desm:"
        },
        {
            "@id": "desm:hasSchema",
            "@type": "rdf:Property",
            "rdfs:label": {"en": "Has Schema"},
            "rdfs:comment": {"en": "Schema in which this property is defined."},
            "rdfs:domain": "rdf:Property",
            "rdfs:range": "desm:Schema",
            "rdfs:isDefinedBy": "desm:"
        },
        {
            "@id": "desm:hasScheme",
            "@type": "rdf:Property",
            "rdfs:label": {"en": "Has Scheme"},
            "rdfs:comment": {"en": "Concept Scheme that belongs to this Data Standards Organization."},
            "rdfs:domain": "desm:DSO",
            "rdfs:range": "skos:ConceptScheme",
            "rdfs:isDefinedBy": "desm:"
        },
        {
            "@id": "desm:hasTermMapping",
            "@type": "rdf:Property" ,       
            "rdfs:label": {"en": "Has Term Mapping"},
            "rdfs:comment": {"en": "Relates a property to a term mapping in which it is included."},
            "rdfs:domain": "rdf:Property",
            "rdfs:range": "desm:TermMapping",
            "rdfs:isDefinedBy": "desm:"
        },
        {
            "@id": "skos:hasTopConcept",
            "@type": "rdf:Property",
            "rdfs:label": {"en": "hasTopCOncept"},
            "rdfs:comment": {"en": "Relates, by convention, a concept scheme to a concept which is topmost in the broader\\/narrower concept hierarchies for that scheme, providing an entry point to these hierarchies."},
            "rdfs:domain": "skos:ConceptScheme",
            "rdfs:range": "skos:Concept",
            "rdfs:isDefinedBy": "skos:"
        },
        {
            "@id": "skos:inScheme",
            "@type": "rdf:Property",
            "rdfs:label": {"en": "In Scheme"},
            "rdfs:comment": {"en": "Relates a resource (for example a concept) to a concept scheme in which it is included."},
            "rdfs:domain": "skos:Concept",
            "rdfs:range": "skos:ConceptScheme",
            "rdfs:isDefinedBy": "skos:"
        },
        {
            "@id": "desm:inSchema",
            "@type": "rdf:Property",
            "rdfs:label": {"en": "In Schema"},
            "rdfs:comment": {"en": "Relates a property to a scheme in which it is included."},
            "rdfs:domain": "rdf:Property",
            "rdfs:range": "desm:Schema",
            "rdfs:isDefinedBy": "desm:"
        },
        {
            "@id": "dct:isPartOf",
            "@type": "rdf:Property",
            "rdfs:label": {"en": "Is Part Of"},
            "rdfs:comment": {"en": "Related resource in which the described resource is physically or logically included."},
            "rdfs:domain": [    
                "desm:TermMapping",
                "desm:AbstractClassMapping"
            ],
            "rdfs:range": [
                "desm:AbstractMapping",
                "desm:AbstractClassSet"
            ],
            "rdfs:isDefinedBy": "dct:"
        },
        {
            "@id": "desm:issue",
            "@type": "rdf:Property",
            "rdfs:label": {"en": "Issue"},
            "rdfs:comment": {"en": "Recording of an issue with mapping a property to another property."},
            "rdfs:domain": "desm:TermMapping",
            "rdfs:range": "rdf:langString",
            "rdfs:isDefinedBy": "desm:"
        },
        {
            "@id": "rdfs:label",
            "@type": "rdf:Property",
            "rdfs:label": {"en": "Human-readable version of the name of a resource."},
            "rdfs:domain": [
                "rdf:Property",
                "rdfs:Class"
            ],
            "rdfs:range": "rdf:langString",
            "rdfs:isDefinedBy": "rdfs:"
        },
        {
            "@id": "desm:mappedTerm",
            "@type": "rdf:Property",
            "rdfs:label": {"en": "Mapped Term"},
            "rdfs:comment": {"en": "Property being mapped to a spine property."},
            "rdfs:domain": "desm:TermMapping",
            "rdfs:range": "rdf:Property",
            "rdfs:isDefinedBy":"desm:"
        },
        {
            "@id": "desm:mapper",
            "@type": "rdf:Property",
            "rdfs:label": {"en": "Mapper"},
            "rdfs:comment": {"en": "An agent adminitering or performing a mapping or crosswalk."},
            "rdfs:domain": "desm:DSO",
            "rdfs:range": "desm:Agent",
            "rdfs:isDefinedBy": "desm:"
        },
        {
            "@id": "desm:mappingPredicate",
            "@type": "rdf:Property",
            "rdfs:label": {"en": "Mapping Predicate"},
            "rdfs:comment": {"en": "Concept identifying the relationship between two properties being mapped."},
            "rdfs:domain": "desm:TermMapping",
            "rdfs:range": "skos:Concept",
            "rdfs:isDefinedBy": "desm:"
        },
        {
            "@id": "desm:mappingPredicateType",
            "@type": "rdf:Property",
            "rdfs:label": {"en": "Mapping Predicate Type"},
            "rdfs:comment": {"en": "Concept scheme defining mapping predicate types."},
            "rdfs:domain": "desm:AbstractCLassSet",
            "rdfs:range": "skos:ConceptScheme",
            "rdfs:isDefinedBy": "desm:"
        },
        {
            "@id": "sdo:name",
            "@type": "rdf:Property",
            "rdfs:label": {"en": "Name"},
            "rdfs:comment": {"en": "The name of the item."},
            "rdfs:domain": "desm:Agent",
            "rdfs:range": "rdf:langString",
            "rdfs:isDefinedBy": "sdo:"
        },
        {
            "@id": "skos:narrower",
            "@type": "rdf:Property",
            "rdfs:label": {"en": "Narrower"}, 
            "rdfs:comment": {"en": "Narrower concepts are typically rendered as children in a concept hierarchy (tree)."},
            "rdfs:domain": "skos:Concept",
            "rdfs:range": "skos:Concept",
            "rdfs:isDefinedBy": "skos:"
        },
        {
            "@id": "desm:range",
            "@type": "rdf:Property",
            "rdfs:label": {"en": "Range"},
            "rdfs:comment": {"en": "Property to used to state that the values of a property are instances of one or more classes."}, 
            "rdfs:domain": "rdf:Property",
            "rdfs:range": [
                "skos:Concept",
                "desm:Class"
            ],
            "rdfs:isDefinedBy": "desm:"
        },
        {
            "@id": "desm:relatedSchema",
            "@type": "rdf:Property",
            "rdfs:label": {"en": "Related Schema"},
            "rdfs:comment": {"en": "Schema to which a concept scheme provides property values."},
            "rdfs:domain": "skos:ConceptSCheme",
            "rdfs:range": "desm:Schema",
            "rdfs:isDefinedBy": "desm:"
        },
        {
            "@id": "desm:role",
            "@type": "rdf:Property",
            "rdfs:label": {"en": "Role"},
            "rdfs:comment": {"en": "Functon or job of an agent."},
            "rdfs:domain": "desm:Agent",
            "rdfs:range": "rdf:langString",
            "rdfs:isDefinedBy": "desm:"
        },
        {
            "@id": "desm:sourcePath",
            "@type": "rdf:Property",
            "rdfs:label": {"en": "Source Path"},
            "rdfs:comment": {"en": "Property or class path in a schema."},
            "rdfs:domain": "rdf:Property",
            "rdfs:range": "xsd:string",
            "rdfs:isDefinedBy": "desm:"
        },
        {
            "@id": "desm:spineTerm",
            "@type": "rdf:Property",
            "rdfs:label": {"en": "Spine Term"},
            "rdfs:comment": {"en": "Property of the synthetic spine generated during the mapping process."},
            "rdfs:domain": {"en": "desm:TermMapping"},
            "rdfs:range": "rdf:Property",
            "rdfs:isDefinedBy": "desm:"
        }
    ]
}
